ConZF.lean
@@ -19,6 +19,7 @@ import ConZF.AllGood
 import ConZF.Lift
 import ConZF.MixedHartogs
 import ConZF.Cofinality
+import ConZF.Interval
 import ConZF.Acc
 import ConZF.CanonicalAcc
 import ConZF.Markov
